an example of eChronos proof firmware

myex/Example.thy
@@ -1,30 +1,73 @@
 theory Example
 imports
-  "../lib/subgoal_focus/Subgoal_Methods"
-  "../lib/Eisbach_Methods"
-  "../lib/Rule_By_Method"
-  (*OG_Bare*)
-  (*OG_Composition*)
-  "../verif/OG_Bare"
-  "../verif/OG_Composition"
+  Example_bare
+  Example_proof_final
 begin
+  
+lemma will_not_fail_merge_prog_list_aux:
+  "same_prog_list_aux TS TS' \<Longrightarrow> merge_prog_list_aux TS TS' = Some (the (merge_prog_list_aux TS TS'))"
+  apply (subst option.collapse)
+   apply (rule ccontr)
+   apply (clarsimp simp: no_merge_imp_not_same_prog_list_aux)
+  apply simp
+  done
+   
     
-record state =
-  x :: nat
+lemma map_eq_conv_length:
+  "length xs = length ys \<Longrightarrow>
+     (map f xs = map f ys) = (\<forall>i<length xs. f (xs ! i) = f (ys ! i))"
+  apply (induct rule: list_induct2)
+   apply simp
+  apply (auto simp add: less_Suc_eq_0_disj)
+  done
     
-definition gg :: "('a state_ext) bare_com"
-  where
-  "gg \<equiv> (COBEGIN
-  \<acute>x:=\<acute>x+1
-  \<parallel>
-  \<acute>x:=\<acute>x+2
-  COEND)"
+lemma extract_ann_prg_merge_prog:
+  "merge_ann_com c c' = Some c'' \<Longrightarrow>
+    extract_ann_prg c'' = extract_ann_prg c"
+  apply (induct c c' arbitrary: c'' rule: merge_ann_com.induct; clarsimp)
+       apply (clarsimp split: if_splits
+            | simp(no_asm_use) split: option.splits)+
+  done
+  
+lemma extract_prg_merge_progI:
+  "same_prog_com c c' \<Longrightarrow>
+   extract_prg c = c'' \<Longrightarrow>
+    extract_prg (the (merge_prog_com c c')) = c''"
+  apply (induct c c' arbitrary: c'' rule: same_prog_com.induct)
+  apply (clarsimp)
+  apply (drule will_not_fail_merge_prog_list_aux)
+  apply (clarsimp split: option.splits)
+  apply (rule conjI)
+  apply (clarsimp)+
+  apply (clarsimp simp: merge_prog_list_aux_def merge_prog_aux_def
+                  split: if_split_asm option.splits)
+  apply (frule those_length[symmetric])
+  apply (drule those_some)
+  apply (clarsimp)
+  apply (clarsimp simp: map_eq_conv_length)
+  apply (drule_tac x=i in spec)
+  apply (clarsimp split: option.splits simp: split_def)[1]
+  apply (erule extract_ann_prg_merge_prog)
+  apply (auto dest: will_not_fail_merge_same_prog_com
+              split: option.splits)
+  done
+    
+lemma same_prog_bare:
+  "extract_prg same_target
+     = target"
+  unfolding same_target_defs
+            target_defs
+  by auto
+  
+lemmas same_prog_bare' =
+          extract_prg_merge_progI[OF same_prog_bare]
   
 lemma p:
-  "\<parallel>-\<^sub>b \<lbrace>True\<rbrace> \<lbrace>True\<rbrace> 
-  gg
-  \<lbrace>True\<rbrace>"
+  "\<parallel>-\<^sub>b \<lbrace>True\<rbrace> \<lbrace>True\<rbrace> target  \<lbrace>True\<rbrace>"
   apply (rule oghoare_bareI)
+  apply (rule exI)
+  apply (rule conjI)
+    apply (rule same_prog_bare')
     oops
   
 end
