myex/Example_bare.thy
@@ -1,0 +1,15 @@
+theory Example_bare
+  imports
+    Example_state
+    "../verif/OG_Bare"
+begin
+  
+definition 
+  target :: "('a state_ext) bare_com"
+where
+  "target \<equiv> \<acute>x:=0"
+  
+lemmas target_defs =
+  target_def
+  
+  end
