myex/Example_proof.thy
@@ -1,0 +1,14 @@
+theory Example_proof
+imports
+    Example_tactic
+begin
+  
+definition same_target
+  where
+    "same_target \<equiv> (\<acute>x:=0)"
+    
+lemmas same_target_defs =
+  same_target_def
+  
+end
+  
