myex/Example_proof_final.thy
@@ -1,0 +1,62 @@
+theory Example_proof_final
+  imports
+    Example_proof
+    "../verif/OG_Composition"
+begin
+  
+lemma will_not_fail_merge_same_prog_com: 
+  "same_prog_com cs cs' \<Longrightarrow> merge_prog_com cs cs' = Some (the (merge_prog_com cs cs'))"
+  apply (subst option.collapse)
+   apply (rule ccontr)
+   apply (clarsimp simp: no_merge_imp_not_same_prog_com)
+  apply simp
+  done
+    
+lemma same_prog_merge''':
+  "same_prog_ann_com p1 p2 \<Longrightarrow>
+   same_prog_ann_com p2 p3 \<Longrightarrow>
+   merge_ann_com p2 p3 = Some p4 \<Longrightarrow>
+   same_prog_ann_com p1 p4"
+  apply (induct p1 p2 arbitrary: p3 p4
+                           rule: same_prog_ann_com.induct; clarsimp)
+       apply (erule same_prog_ann_com.elims; fastforce split: option.splits)+
+  done
+    
+lemma same_prog_merge'':
+  "\<lbrakk>same_prog_aux (a, b) (aa, ba); same_prog_aux (aa, ba) (ab, bb);
+        merge_prog_aux (aa, ba) (ab, bb) = Some (ac, bc)\<rbrakk>
+       \<Longrightarrow> same_prog_aux (a, b) (ac, bc)"
+  apply (clarsimp simp: same_prog_aux_def merge_prog_aux_def)
+  apply (clarsimp split: option.splits)
+  apply (drule_tac s="Some _" in sym)
+  apply clarsimp
+  apply (rule same_prog_merge'''; simp)
+  done
+    
+lemma same_prog_merge':
+  "\<lbrakk>same_prog_list_aux Ts Ts'; same_prog_list_aux Ts' Ts'';
+        merge_prog_list_aux Ts' Ts'' = Some Ts'''\<rbrakk>
+       \<Longrightarrow> same_prog_list_aux Ts Ts'''"
+  apply (clarsimp simp: same_prog_list_aux_def merge_prog_list_aux_def)
+  apply (induct Ts arbitrary: Ts' Ts'' Ts'''; simp)
+  apply (clarsimp simp: zip_Cons1 split: list.splits option.splits)
+  apply (rule same_prog_merge''; simp)
+  done
+    
+lemma same_prog_merge:
+  "same_prog_com p1 p2 \<Longrightarrow>
+   same_prog_com p2 p3 \<Longrightarrow>
+   same_prog_com p1 (the (merge_prog_com p2 p3))"
+  apply (frule will_not_fail_merge_same_prog_com)
+  apply (frule_tac cs=p2 in will_not_fail_merge_same_prog_com)
+  apply (induct p1 p2 arbitrary: p3 rule: same_prog_com.induct; simp)
+      apply (erule same_prog_com.elims; clarsimp split: option.splits)
+      apply (rule same_prog_merge'; simp)
+     apply (erule same_prog_com.elims; fastforce split: option.splits)+
+  done
+    
+lemmas same_prog_all_invs =
+  same_prog_merge[]
+  
+end
+  
