myex/Example_state.thy
@@ -1,0 +1,28 @@
+theory Example_state
+  imports
+    "../lib/Rule_By_Method"
+begin
+  
+record state =
+  x :: nat
+  
+locale foo
+  =
+  fixes Red :: "'a state_scheme"
+begin
+  
+lemmas r_surj = state.surjective[of Red,symmetric]
+  
+lemmas foo = 
+  state.update_convs[of "\<lambda>_. X" for X, @ (schematic) \<open>subst (asm) r_surj\<close>,symmetric]
+  
+lemmas foo' = state.select_convs(1) select_convs
+  
+lemmas foos = foo'[@ (schematic) \<open>subst (asm) foo(1)\<close>]
+  
+end
+  
+lemmas state_upd_simps = foo.foos
+  
+end
+  
