myex/Example_tactic.thy
@@ -1,0 +1,93 @@
+theory Example_tactic
+
+imports
+  "../verif/OG_More"
+  Example_state
+  "../lib/Hoare_Parallel/OG_Syntax"
+  "../lib/subgoal_focus/Subgoal_Methods"
+  "../lib/Eisbach_Methods"
+begin
+
+ML \<open>
+fun timed_tac i ctxt st seq =
+  let
+    fun str_of_goal th = Pretty.string_of (Goal_Display.pretty_goal ctxt th)
+
+    fun limit f x = Timeout.apply (Time.fromSeconds i) f x
+      handle Timeout.TIMEOUT _ =>
+        let val _ = warning ("Method timed out:\n"(* ^ (str_of_goal st)*))
+        in SOME (st, Seq.empty) end
+  in
+    Seq.make (limit (fn () => Option.map (apsnd (timed_tac i ctxt st))
+      (Seq.pull seq)))
+  end
+\<close>
+
+ML \<open>
+(*Apply second tactic to all subgoals emerging from the first,
+  but not the last one --
+  following usual convention for subgoal-based tactics.*)
+infix 1 THEN_ALL_NEW_BUT_1;
+
+fun (tac1 THEN_ALL_NEW_BUT_1 tac2) i st =
+  st |> (tac1 i THEN (fn st' =>
+    Seq.INTERVAL tac2 i (i + Thm.nprems_of st' - Thm.nprems_of st - 1) st'));
+
+fun DETERM' tac i = DETERM (tac i)
+
+fun TRY' tac i = TRY (tac i)
+
+fun TRY_EVERY' tacs i = EVERY' (map (fn tac => TRY' tac) tacs) i
+
+fun FORWARD tac ctxt = tac THEN_ALL_NEW_BUT_1 (SOLVED' (assume_tac ctxt))
+
+fun TRY_EVERY_FORWARD' ctxt thms i =
+  TRY_EVERY' (map (fn thm => FORWARD (forward_tac ctxt [thm]) ctxt) thms) i
+\<close>
+  
+lemma last_single:
+  "last [x] = x"
+  by simp
+    
+lemmas subset_eqI = subset_eq[THEN iffD2]
+  
+lemma
+  union_negI_drop: 
+  "x \<in> A \<Longrightarrow> x \<in> A \<union> -B"
+  by blast
+    
+lemma CollectNotD: "a \<notin> {x. P x} \<Longrightarrow> \<not> P a"
+  by simp
+
+ML \<open>
+fun set_to_logic ctxt i =
+  let val simp_ctxt = ((clear_simpset ctxt)
+          addsimps @{thms state_upd_simps HOL.simp_thms HOL.all_simps HOL.ex_simps
+                          option.inject pre.simps snd_conv option.sel last_single
+                          neq_Nil_conv 
+                          (*U_simps svc\<^sub>a_commute handle_events_empty*)
+                          })
+                  |> Splitter.add_split @{thm if_split_asm}
+                  |> Splitter.add_split @{thm if_split}
+  in DETERM (REPEAT_ALL_NEW (resolve_tac ctxt
+                  @{thms subset_eqI subsetI ballI CollectI IntI conjI disjCI impI
+                         union_negI_drop}
+         ORELSE' DETERM o dresolve_tac ctxt @{thms CollectD Set.singletonD
+                                                   ComplD CollectNotD
+                                                   Meson.not_conjD
+                                                   Meson.not_exD
+                                                   set_ConsD}
+         ORELSE' DETERM o eresolve_tac ctxt @{thms IntE conjE exE insertE}
+         ORELSE' CHANGED o safe_asm_full_simp_tac simp_ctxt
+         ORELSE' CHANGED o Classical.clarify_tac (Clasimp.addSss simp_ctxt)) i)
+  end
+
+(*fun svc_commute ctxt =
+  ((TRY' o REPEAT_ALL_NEW) ((EqSubst.eqsubst_tac ctxt [0] @{thms svc\<^sub>a_commute})
+                ORELSE' (EqSubst.eqsubst_asm_tac ctxt [0] @{thms svc\<^sub>a_commute})))
+  THEN'
+  ((TRY' o REPEAT_ALL_NEW) ((EqSubst.eqsubst_tac ctxt [0] @{thms svc\<^sub>s_commute})
+                ORELSE' (EqSubst.eqsubst_asm_tac ctxt [0] @{thms svc\<^sub>s_commute})))*)
+\<close>
+
+end
